feat: Expr.WF and unique typing

Lean4Lean/Theory/Typing/Basic.lean
@@ -66,7 +66,12 @@ def HasType (env : VEnv) (U : Nat) (Γ : List VExpr) (e A : VExpr) : Prop :=
 def IsType (env : VEnv) (U : Nat) (Γ : List VExpr) (A : VExpr) : Prop :=
   ∃ u, env.HasType U Γ A (.sort u)
 
+def IsDefEqU (env : VEnv) (U : Nat) (Γ : List VExpr) (e₁ e₂ : VExpr) :=
+  ∃ A, env.IsDefEq U Γ e₁ e₂ A
+
 end VEnv
+
+def VExpr.WF (env : VEnv) (U : Nat) (Γ : List VExpr) (e : VExpr) := env.IsDefEqU U Γ e e
 
 def VConstant.WF (env : VEnv) (ci : VConstant) : Prop := env.IsType ci.uvars [] ci.type
 
