Lean4Lean/Verify/Typing/Expr.lean
@@ -1,0 +1,61 @@
+import Lean4Lean.Theory.Typing.Basic
+import Lean4Lean.Verify.VLCtx
+
+namespace Lean4Lean
+open Lean
+
+variable (fvars : List FVarId) in
+def InScope : Expr → (k :_:= 0) → Prop
+  | .bvar i, k => i < k
+  | .fvar fv, _ => fv ∈ fvars
+  | .sort .., _ | .const .., _ | .lit .., _ => True
+  | .app f a, k => InScope f k ∧ InScope a k
+  | .lam _ d b _, k
+  | .forallE _ d b _, k => InScope d k ∧ InScope b (k+1)
+  | .letE _ d v b _, k => InScope d k ∧ InScope v k ∧ InScope b (k+1)
+  | .proj _ _ e, k | .mdata _ e, k => InScope e k
+  | .mvar .., _ => False
+
+def VLocalDecl.WF (env : VEnv) (U : Nat) (Δ : VLCtx) : VLocalDecl → Prop
+  | .vlam type => env.IsType U Δ.toCtx type
+  | .vlet type value => env.HasType U Δ.toCtx value type
+
+variable (env : VEnv) (U : Nat) in
+def VLCtx.WF : VLCtx → Prop
+  | [] => True
+  | (ofv, d) :: (Δ : VLCtx) =>
+    VLCtx.WF Δ ∧ (do Δ.lookup (some (← ofv))) = none ∧ VLocalDecl.WF env U Δ d
+
+def TrProj (Δ : VLCtx) (structName : Name) (idx : Nat) (e : VExpr) : VExpr → Prop := sorry
+
+variable (env : VEnv) (Us : List Name) in
+inductive TrExpr : VLCtx → Expr → VExpr → Prop
+  | bvar : Δ.find? (.inl i) = some (d, n) → TrExpr Δ (.bvar i) (d.value.liftN n)
+  | fvar : Δ.find? (.inr fv) = some (d, n) → TrExpr Δ (.fvar fv) (d.value.liftN n)
+  | sort : VLevel.ofLevel Us u = some u' → TrExpr Δ (.sort u) (.sort u')
+  | const :
+    env.constants c = some (some ci) →
+    us.mapM (VLevel.ofLevel Us) = some us' →
+    us.length = ci.uvars →
+    TrExpr Δ (.const c us) (.const c us')
+  | app :
+    env.HasType Us.length Δ.toCtx f' (.forallE A B) →
+    env.HasType Us.length Δ.toCtx a' A →
+    TrExpr Δ f f' → TrExpr Δ a a' → TrExpr Δ (.app f a) (.app f' a')
+  | lam :
+    env.IsType Us.length Δ.toCtx ty' →
+    TrExpr Δ ty ty' → TrExpr ((none, .vlam ty') :: Δ) body body' →
+    TrExpr Δ (.lam name ty body bi) (.lam ty' body')
+  | forallE :
+    env.IsType Us.length Δ.toCtx ty' →
+    env.IsType Us.length (ty' :: Δ.toCtx) body' →
+    TrExpr Δ ty ty' → TrExpr ((none, .vlam ty') :: Δ) body body' →
+    TrExpr Δ (.forallE name ty body bi) (.forallE ty' body')
+  | letE :
+    env.HasType Us.length Δ.toCtx val' ty' →
+    TrExpr Δ ty ty' → TrExpr Δ val val' →
+    TrExpr ((none, .vlet ty' val') :: Δ) body body' →
+    TrExpr Δ (.letE name ty val body bi) body'
+  | lit : TrExpr Δ l.toConstructor e → TrExpr Δ (.lit l) e
+  | mdata : TrExpr Δ e e' → TrExpr Δ (.mdata d e) e'
+  | proj : TrExpr Δ e e' → TrProj Δ s i e' e'' → TrExpr Δ (.proj s i e) e''
