Lean4Lean/Verify/Typing/Lemmas.lean
@@ -1,0 +1,184 @@
+import Lean4Lean.Verify.Typing.Expr
+import Lean4Lean.Theory.Typing.Strong
+import Lean4Lean.Theory.Typing.UniqueTyping
+
+namespace Lean4Lean
+open VEnv
+
+theorem VLocalDecl.WF.hasType :
+    ∀ {d}, VLocalDecl.WF env U Δ d → env.HasType U (VLCtx.toCtx ((ofv, d) :: Δ)) d.value d.type
+  | .vlam _, _ => .bvar .zero
+  | .vlet .., hA => hA
+
+theorem VLCtx.WF.find?_wf' {Δ : VLCtx} (hΔ : VLCtx.WF env U Δ) (H : Δ.find? v = some (d, n)) :
+    ∃ Γ Γ', Δ.toCtx = Γ' ++ Γ ∧ Γ'.length = n ∧ env.HasType U Γ d.value d.type := by
+  let (ofv, d') :: Δ := Δ
+  unfold VLCtx.find? at H; split at H
+  · cases H; exact ⟨_, [], by simp; rfl, rfl, hΔ.2.2.hasType⟩
+  · simp [bind, Option.bind_eq_some] at H
+    obtain ⟨⟨d'', n'⟩, H, rfl, h2⟩ := H
+    obtain ⟨Γ, Γ', h1, rfl, h3⟩ := hΔ.1.find?_wf' H
+    match d' with
+    | .vlam A => exact ⟨Γ, A::Γ', congrArg (A::·) h1, h2, h3⟩
+    | .vlet e A => exact ⟨Γ, Γ', h1, h2, h3⟩
+
+variable (henv : Ordered env) in
+theorem VLCtx.WF.find?_wf {Δ : VLCtx} (hΔ : VLCtx.WF env U Δ) (H : Δ.find? v = some (d, n)) :
+    env.HasType U Δ.toCtx (d.value.liftN n) (d.type.liftN n) :=
+  let ⟨_, _, h1, h2, h3⟩ := hΔ.find?_wf' H; h3.weakN henv (h1 ▸ .zero _ h2)
+
+theorem VLCtx.WF.toCtx : ∀ {Δ}, VLCtx.WF env U Δ → OnCtx Δ.toCtx (env.IsType U)
+  | [], _ => ⟨⟩
+  | (_, .vlam _) :: _, ⟨hΔ, _, hA⟩ => ⟨hΔ.toCtx, hA⟩
+  | (_, .vlet ..) :: _, ⟨hΔ, _, _⟩ => hΔ.toCtx
+
+variable (env : VEnv) (U : Nat) in
+inductive VLCtx.IsDefEq : VLCtx → VLCtx → Prop
+  | nil : VLCtx.IsDefEq [] []
+  | vlam {Δ₁ Δ₂ : VLCtx} :
+    VLCtx.IsDefEq Δ₁ Δ₂ →
+    (do Δ₁.lookup (some (← ofv))) = none →
+    env.IsDefEq U Δ₁.toCtx type₁ type₂ (.sort u) →
+    VLCtx.IsDefEq ((ofv, .vlam type₁) :: Δ₁) ((ofv, .vlam type₂) :: Δ₂)
+  | vlet {Δ₁ Δ₂ : VLCtx} :
+    VLCtx.IsDefEq Δ₁ Δ₂ →
+    (do Δ₁.lookup (some (← ofv))) = none →
+    env.IsDefEq U Δ₁.toCtx value₁ value₂ type₁ →
+    env.IsDefEq U Δ₁.toCtx type₁ type₂ (.sort u) →
+    VLCtx.IsDefEq ((ofv, .vlet type₁ value₁) :: Δ₁) ((ofv, .vlet type₂ value₂) :: Δ₂)
+
+variable (henv : Ordered env) in
+theorem VLCtx.IsDefEq.refl : ∀ {Δ}, VLCtx.WF env U Δ → VLCtx.IsDefEq env U Δ Δ
+  | [], _ => .nil
+  | (_, .vlam ..) :: _, ⟨h1, h2, _, h3⟩ => .vlam (IsDefEq.refl h1) h2 h3
+  | (_, .vlet ..) :: _, ⟨h1, h2, h3⟩ =>
+    let ⟨_, h4⟩ := h3.isType henv h1.toCtx
+    .vlet (IsDefEq.refl h1) h2 h3 h4
+
+theorem VLCtx.IsDefEq.defeqCtx : VLCtx.IsDefEq env U Δ₁ Δ₂ → env.IsDefEqCtx U [] Δ₁.toCtx Δ₂.toCtx
+  | .nil => .zero
+  | .vlam h1 _ h3 => .succ h1.defeqCtx h3
+  | .vlet h1 _ _ _ => h1.defeqCtx
+
+theorem VLCtx.IsDefEq.lookup_eq_none :
+    VLCtx.IsDefEq env U Δ₁ Δ₂ → (Δ₁.lookup fv = none ↔ Δ₂.lookup fv = none)
+  | .nil => by simp
+  | .vlam h1 _ _ | .vlet h1 _ _ _ => by simp [List.lookup]; split <;> simp [h1.lookup_eq_none]
+
+theorem VLCtx.IsDefEq.find? :
+    VLCtx.IsDefEq env U Δ₁ Δ₂ → (Δ₁.lookup fv = none ↔ Δ₂.lookup fv = none)
+  | .nil => by simp
+  | .vlam h1 _ _ | .vlet h1 _ _ _ => by simp [List.lookup]; split <;> simp [h1.lookup_eq_none]
+
+theorem VLCtx.IsDefEq.bind_lookup_eq_none (H : VLCtx.IsDefEq env U Δ₁ Δ₂) :
+    (do Δ₁.lookup (some (← ofv))) = none ↔ (do Δ₂.lookup (some (← ofv))) = none := by
+  simp only [bind, Option.bind_eq_none]
+  repeat rw [forall_comm, forall_comm (α := VLocalDecl)]; refine forall_congr' fun _ => ?_
+  simp only [← Option.eq_none_iff_forall_not_mem, H.lookup_eq_none]
+
+theorem VLCtx.IsDefEq.wf : VLCtx.IsDefEq env U Δ₁ Δ₂ → VLCtx.WF env U Δ₁
+  | .nil => ⟨⟩
+  | .vlam h1 h2 h3 => ⟨h1.wf, h2, _, h3.hasType.1⟩
+  | .vlet h1 h2 h3 _ => ⟨h1.wf, h2, h3.hasType.1⟩
+
+variable (henv : Ordered env) in
+theorem VLCtx.IsDefEq.symm : VLCtx.IsDefEq env U Δ₁ Δ₂ → VLCtx.IsDefEq env U Δ₂ Δ₁
+  | .nil => .nil
+  | .vlam h1 h2 h3 =>
+    .vlam h1.symm (by simpa [h1.bind_lookup_eq_none] using h2) (h3.symm.defeqDFC henv h1.defeqCtx)
+  | .vlet h1 h2 h3 h4 =>
+    .vlet h1.symm (by simpa [h1.bind_lookup_eq_none] using h2)
+      (h4.defeqDF h3.symm |>.defeqDFC henv h1.defeqCtx) (h4.symm.defeqDFC henv h1.defeqCtx)
+
+theorem VLCtx.IsDefEq.find?_uniq' (hΔ : VLCtx.IsDefEq env U Δ₁ Δ₂)
+    (H1 : Δ₁.find? v = some (d₁, n₁)) (H2 : Δ₂.find? v = some (d₂, n₂)) :
+    ∃ Γ₁ Γ₁', Δ₁.toCtx = Γ₁' ++ Γ₁ ∧ Γ₁'.length = n₁ ∧
+    ∃ Γ₂ Γ₂', Δ₂.toCtx = Γ₂' ++ Γ₂ ∧ Γ₂'.length = n₂ ∧
+    n₁ = n₂ ∧ env.IsDefEq U Γ₁ d₁.value d₂.value d₁.type := by
+  match hΔ with
+  | .vlam (type₁ := A₁) (type₂ := A₂) hΔ h2 h3 =>
+    revert H1 H2; unfold VLCtx.find?; split
+    · rintro ⟨⟩ ⟨⟩
+      exact ⟨_, [], rfl, rfl, _, [], rfl, rfl, rfl, .bvar .zero⟩
+    · simp [bind, Option.bind_eq_some]
+      rintro ⟨d₁', n₁'⟩ H1' rfl rfl ⟨d₂', n₂'⟩ H2' rfl rfl
+      obtain ⟨Γ₁, Γ₁', h1, rfl, Γ₂, Γ₂', h2, rfl, eq, h3⟩ := find?_uniq' hΔ H1' H2'
+      exact ⟨
+        Γ₁, A₁::Γ₁', congrArg (_::·) h1, rfl,
+        Γ₂, A₂::Γ₂', congrArg (_::·) h2, rfl,
+        congrArg Nat.succ eq, h3⟩
+  | .vlet hΔ _ h3 _ =>
+    revert H1 H2; unfold VLCtx.find?; split
+    · rintro ⟨⟩ ⟨⟩
+      exact ⟨_, [], rfl, rfl, _, [], rfl, rfl, rfl, h3⟩
+    · simp [bind, Option.bind_eq_some]
+      rintro ⟨d₁', n₁'⟩ H1' rfl rfl ⟨d₂', n₂'⟩ H2' rfl rfl
+      exact (find?_uniq' hΔ H1' H2' :)
+
+variable (henv : Ordered env) in
+theorem VLCtx.IsDefEq.find?_uniq (hΔ : VLCtx.IsDefEq env U Δ₁ Δ₂)
+    (H1 : Δ₁.find? v = some (d₁, n₁)) (H2 : Δ₂.find? v = some (d₂, n₂)) :
+    n₁ = n₂ ∧
+    env.IsDefEq U Δ₁.toCtx (d₁.value.liftN n₁) (d₂.value.liftN n₂) (d₁.type.liftN n₁) := by
+  obtain ⟨_, _, h1, rfl, _, _, _, _, eq, h3⟩ := find?_uniq' hΔ H1 H2
+  exact ⟨eq, eq ▸ h3.weakN henv (h1 ▸ .zero _)⟩
+
+theorem TrProj.wf (H1 : TrProj Δ s i e e') (H2 : VExpr.WF env U Γ e) : VExpr.WF env U Γ e' := sorry
+
+variable (henv : Ordered env) {Us : List Name} (hΔ : VLCtx.WF env Us.length Δ) in
+theorem TrExpr.wf (H : TrExpr env Us Δ e e') : VExpr.WF env Us.length Δ.toCtx e' := by
+  induction H with
+  | bvar h1 | fvar h1 => exact ⟨_, hΔ.find?_wf henv h1⟩
+  | sort h1 => exact ⟨_, .sort (.of_ofLevel h1)⟩
+  | const h1 h2 h3 =>
+    simp [List.mapM_eq_some] at h2
+    refine ⟨_, .const h1 (fun l hl => ?_) (h2.length_eq.symm.trans h3)⟩
+    have ⟨_, _, h⟩ := h2.forall_exists_r _ hl; exact .of_ofLevel h
+  | app h1 h2 => exact ⟨_, .app h1 h2⟩
+  | lam h1 _ _ _ ih2 =>
+    have ⟨_, h1'⟩ := h1
+    have ⟨_, h2'⟩ := ih2 ⟨hΔ, rfl, h1⟩
+    refine ⟨_, .lam h1' h2'⟩
+  | forallE h1 h2 => have ⟨_, h1'⟩ := h1; have ⟨_, h2'⟩ := h2; exact ⟨_, .forallE h1' h2'⟩
+  | letE h1 _ _ _ _ _ ih3 => exact ih3 ⟨hΔ, rfl, h1⟩
+  | lit _ ih | mdata _ ih => exact ih hΔ
+  | proj _ h2 ih => exact h2.wf (ih hΔ)
+
+variable (henv : Ordered env) (hΔ : VLCtx.IsDefEq env U Δ₁ Δ₂) in
+theorem TrProj.uniq (H1 : TrProj Δ₁ s i e₁ e₁') (H2 : TrProj Δ₂ s i e₂ e₂')
+    (H : env.IsDefEqU U Δ₁.toCtx e₁ e₂) :
+    env.IsDefEqU U Δ₁.toCtx e₁' e₂' := sorry
+
+variable (henv : Ordered env) (Us : List Name) (hΔ : VLCtx.IsDefEq env Us.length Δ₁ Δ₂) in
+theorem TrExpr.uniq (H1 : TrExpr env Us Δ₁ e e₁) (H2 : TrExpr env Us Δ₂ e e₂) :
+    env.IsDefEqU Us.length Δ₁.toCtx e₁ e₂ := by
+  induction H1 generalizing Δ₂ e₂ with
+  | bvar l1 => let .bvar r1 := H2; obtain ⟨rfl, h⟩ := hΔ.find?_uniq henv l1 r1; exact ⟨_, h⟩
+  | fvar l1 => let .fvar r1 := H2; obtain ⟨rfl, h⟩ := hΔ.find?_uniq henv l1 r1; exact ⟨_, h⟩
+  | sort l1 => let .sort r1 := H2; cases l1.symm.trans r1; exact ⟨_, .sort (.of_ofLevel l1)⟩
+  | const l1 l2 l3 =>
+    let .const r1 r2 r3 := H2; cases l1.symm.trans r1; cases l2.symm.trans r2
+    exact (TrExpr.const l1 l2 l3).wf henv hΔ.wf
+  | app l1 l2 _ _ ih3 ih4 =>
+    let .app _ _ r3 r4 := H2
+    exact ⟨_, .appDF
+      (ih3 hΔ r3 |>.of_l henv hΔ.wf.toCtx l1)
+      (ih4 hΔ r4 |>.of_l henv hΔ.wf.toCtx l2)⟩
+  | lam l1 _ _ ih2 ih3 =>
+    let ⟨_, l1⟩ := l1; let .lam _ r2 r3 := H2
+    have hA := ih2 hΔ r2 |>.of_l henv hΔ.wf.toCtx l1
+    have ⟨_, hb⟩ := ih3 (hΔ.vlam rfl hA) r3
+    exact ⟨_, .lamDF hA hb⟩
+  | forallE l1 l2 _ _ ih3 ih4 =>
+    let ⟨_, l1'⟩ := l1; let ⟨_, l2⟩ := l2; let .forallE _ _ r3 r4 := H2
+    have hA := ih3 hΔ r3 |>.of_l henv hΔ.wf.toCtx l1'
+    have hB := ih4 (.vlam hΔ rfl hA) r4 |>.of_l (Γ := _::_) henv ⟨hΔ.wf.toCtx, l1⟩ l2
+    exact ⟨_, .forallEDF hA hB⟩
+  | letE l1 _ _ _ ih2 ih3 ih4 =>
+    have hΓ := hΔ.wf.toCtx
+    let .letE _ r2 r3 r4 := H2
+    have ⟨_, hb⟩ := l1.isType henv hΓ
+    exact ih4 (.vlet hΔ rfl (ih3 hΔ r3 |>.of_l henv hΓ l1) (ih2 hΔ r2 |>.of_l henv hΓ hb)) r4
+  | lit _ ih1 => let .lit r1 := H2; exact ih1 hΔ r1
+  | mdata _ ih1 => let .mdata r1 := H2; exact ih1 hΔ r1
+  | proj _ l2 ih1 => let .proj r1 r2 := H2; exact l2.uniq r2 (ih1 hΔ r1)
