Lean4Lean/Verify/VLCtx.lean
@@ -1,0 +1,53 @@
+import Lean4Lean.Expr
+import Lean4Lean.Theory.VExpr
+
+namespace Lean4Lean
+
+open Lean (FVarId Expr)
+
+inductive VLocalDecl where
+  | vlam (type : VExpr)
+  | vlet (type value : VExpr)
+
+def VLocalDecl.depth : VLocalDecl → Nat
+  | .vlam .. => 1
+  | .vlet .. => 0
+
+def VLocalDecl.value : VLocalDecl → VExpr
+  | .vlam .. => .bvar 0
+  | .vlet _ e => e
+
+def VLocalDecl.type' : VLocalDecl → VExpr
+  | .vlam A
+  | .vlet A _ => A
+
+def VLocalDecl.type : VLocalDecl → VExpr
+  | .vlam A => A.lift
+  | .vlet A _ => A
+
+def VLCtx := List (Option FVarId × VLocalDecl)
+
+namespace VLCtx
+
+def next : Option FVarId → Nat ⊕ FVarId → Option (Nat ⊕ FVarId)
+  | none, .inl 0 => none
+  | none, .inl (n+1) => some (.inl n)
+  | some _, .inl n => some (.inl n)
+  | none, .inr fv' => some (.inr fv')
+  | some fv, .inr fv' => if fv == fv' then none else some (.inr fv')
+
+def find? : VLCtx → Nat ⊕ FVarId → Option (VLocalDecl × Nat)
+  | [], _ => none
+  | (ofv, d) :: Δ, v =>
+    match next ofv v with
+    | none => some (d, 0)
+    | some v => do let (d', i) ← find? Δ v; some (d', i + d.depth)
+
+def fvars (Δ : VLCtx) : List FVarId := Δ.filterMap (·.1)
+
+def toCtx : VLCtx → List VExpr
+  | [] => []
+  | (_, .vlam ty) :: Δ => ty :: VLCtx.toCtx Δ
+  | (_, .vlet _ _) :: Δ => VLCtx.toCtx Δ
+
+end VLCtx
